src/cddl/pulse/CDDL.Pulse.Serialize.Gen.MapGroup.ZeroOrMore.Aux2.Lemma8.fsti
@@ -29,7 +29,8 @@ val invariant_count_overflow
   (max: option nat)
 : Lemma
   (requires
-    impl_serialize_map_zero_or_more_iterator_gen_invariant p sp1 sp2 except em out vout size count m v0 v min max true
+    impl_serialize_map_zero_or_more_iterator_gen_invariant p sp1 sp2 except em out vout size count m v0 v min max true /\
+    U64.v count == pow2 64 - 1
   )
   (ensures
     impl_serialize_map_zero_or_more_iterator_gen_invariant p sp1 sp2 except em out vout size count m v0 v min max false
